clean up atomic triple def

atomic/invariant.v
@@ -1,7 +1,8 @@
 From stdpp Require Import namespaces.
 From iris.bi.lib Require Export atomic.
 From iris.proofmode Require Import proofmode.
-
+From iris.program_logic Require Export weakestpre.
+From iris.base_logic Require Import invariants.
 
 Section definition.
   Context {PROP : bi} `{!BiFUpd PROP} {TA TB : tele}.
@@ -12,25 +13,93 @@ Section definition.
     (Φ : TA → TB → PROP) (* post-condition *)
   .
   
-  Definition atomic_resource Eo Ei α Φ := (λ x y,
-    atomic_update Eo Ei α (λ (x : TA) (_ : TB), α x) (λ (_ : TA) (_ : TB), Φ x y))%I.
+  Definition atomic_resource Eo Ei α Ψ :=  
+    atomic_update Eo Ei α (λ (x : TA) (_ : TA), α x) (λ (_ : TA) (_ : TA), Ψ).
   Definition atomic_invariant Eo Ei α β Φ :=
-    atomic_update Eo Ei α β (atomic_resource Eo Ei α Φ).
+    atomic_update Eo Ei α β (λ x y, atomic_resource Eo Ei α (Φ x y)).
 
-  Lemma ainv_aupd Eo Ei α β Φ :
-    atomic_update Eo Ei α β (atomic_resource Eo Ei α Φ) -∗
+  Local Lemma ainv_aupd Eo Ei α β Φ :
+    atomic_update Eo Ei α β (λ x y, atomic_resource Eo Ei α (Φ x y)) -∗
     atomic_invariant Eo Ei α β Φ.
   Proof. by iIntros. Qed.
 
-  Lemma ares_aupd Eo Ei α Φ x y :
-    atomic_update Eo Ei α (λ (x : TA) (_ : TB), α x) (λ (_ : TA) (_ : TB), Φ x y) -∗
-    atomic_resource Eo Ei α Φ x y.
+  Local Lemma ares_aupd Eo Ei α Ψ :
+    atomic_update Eo Ei α (λ (x : TA) (_ : TA), α x) (λ (_ : TA) (_ : TA), Ψ) -∗
+    atomic_resource Eo Ei α Ψ.
   Proof. by iIntros. Qed.
 End definition.
 
+(** Notation: Atomic invariants *)
+Notation "'AI' '<{' ∃∃ x1 .. xn , α '}>' @ Eo , Ei '<{' ∀∀ y1 .. yn , β , 'COMM' Φ '}>'" :=
+  (atomic_invariant (TA:=TeleS (λ x1, .. (TeleS (λ xn, TeleO)) .. ))
+                (TB:=TeleS (λ y1, .. (TeleS (λ yn, TeleO)) .. ))
+                Eo Ei
+                (tele_app $ λ x1, .. (λ xn, α%I) ..)
+                (tele_app $ λ x1, .. (λ xn,
+                        tele_app (λ y1, .. (λ yn, β%I) .. )
+                        ) .. )
+                (tele_app $ λ x1, .. (λ xn,
+                        tele_app (λ y1, .. (λ yn, Φ%I) .. )
+                        ) .. )
+  )
+  (at level 20, Eo, Ei, α, β, Φ at level 200, x1 binder, xn binder, y1 binder, yn binder,
+  format "'[hv   ' 'AI'  '<{'  '[' ∃∃  x1  ..  xn ,  '/' α  ']' '}>'  '/' @  '[' Eo ,  '/' Ei ']'  '/' '<{'  '[' ∀∀  y1  ..  yn ,  '/' β ,  '/' COMM  Φ  ']' '}>' ']'") : bi_scope.
+
+Notation "'AI' '<{' ∃∃ x1 .. xn , α '}>' @ Eo , Ei '<{' β , 'COMM' Φ '}>'" :=
+  (atomic_invariant (TA:=TeleS (λ x1, .. (TeleS (λ xn, TeleO)) .. ))
+                (TB:=TeleO)
+                Eo Ei
+                (tele_app $ λ x1, .. (λ xn, α%I) ..)
+                (tele_app $ λ x1, .. (λ xn, tele_app β%I) .. )
+                (tele_app $ λ x1, .. (λ xn, tele_app Φ%I) .. )
+  )
+  (at level 20, Eo, Ei, α, β, Φ at level 200, x1 binder, xn binder,
+  format "'[hv   ' 'AI'  '<{'  '[' ∃∃  x1  ..  xn ,  '/' α  ']' '}>'  '/' @  '[' Eo ,  '/' Ei ']'  '/' '<{'  '[' β ,  '/' COMM  Φ  ']' '}>' ']'") : bi_scope.
+
+Notation "'AI' '<{' α '}>' @ Eo , Ei '<{' ∀∀ y1 .. yn , β , 'COMM' Φ '}>'" :=
+  (atomic_invariant (TA:=TeleO)
+                (TB:=TeleS (λ y1, .. (TeleS (λ yn, TeleO)) .. ))
+                Eo Ei
+                (tele_app α%I)
+                (tele_app $ tele_app (λ y1, .. (λ yn, β%I) ..))
+                (tele_app $ tele_app (λ y1, .. (λ yn, Φ%I) ..))
+  )
+  (at level 20, Eo, Ei, α, β, Φ at level 200, y1 binder, yn binder,
+  format "'[hv   ' 'AI'  '<{'  '[' α  ']' '}>'  '/' @  '[' Eo ,  '/' Ei ']'  '/' '<{'  '[' ∀∀  y1  ..  yn ,  '/' β ,  '/' COMM  Φ  ']' '}>' ']'") : bi_scope.
+
+Notation "'AI' '<{' α '}>' @ Eo , Ei '<{' β , 'COMM' Φ '}>'" :=
+  (atomic_invariant (TA:=TeleO) (TB:=TeleO)
+                Eo Ei
+                (tele_app α%I)
+                (tele_app $ tele_app β%I)
+                (tele_app $ tele_app Φ%I)
+  )
+  (at level 20, Eo, Ei, α, β, Φ at level 200,
+  format "'[hv   ' 'AI'  '<{'  '[' α  ']' '}>'  '/' @  '[' Eo ,  '/' Ei ']'  '/' '<{'  '[' β ,  '/' COMM  Φ  ']' '}>' ']'") : bi_scope.
+
+(** Notation: Atomic resources *)
+Notation "'AR' '<{' ∃∃ x1 .. xn , α '}>' @ Eo , Ei '<{' Ψ '}>'" :=
+  (atomic_resource (TA:=TeleS (λ x1, .. (TeleS (λ xn, TeleO)) .. ))
+                Eo Ei
+                (tele_app $ λ x1, .. (λ xn, α%I) ..)
+                (tele_app Ψ%I)
+  )
+  (at level 20, Eo, Ei, α, Ψ at level 200, x1 binder, xn binder,
+  format "'[hv   ' 'AR'  '<{'  '[' ∃∃  x1  ..  xn ,  '/' α  ']' '}>'  '/' @  '[' Eo ,  '/' Ei ']'  '/' '<{'  '['  Ψ  ']' '}>' ']'") : bi_scope.
+
+Notation "'AR' '<{' α '}>' @ Eo , Ei '<{' Ψ '}>'" :=
+  (atomic_resource (TA:=TeleO)
+                Eo Ei
+                (tele_app α%I)
+                (tele_app Ψ%I)
+  )
+  (at level 20, Eo, Ei, α, Ψ at level 200,
+  format "'[hv   ' 'AR'  '<{'  '[' α  ']' '}>'  '/' @  '[' Eo ,  '/' Ei ']'  '/' '<{'  '['  Ψ  ']' '}>' ']'") : bi_scope.
+
 Section properties.
-  Context `{BiFUpd PROP} {TA TB : tele}.
-  Implicit Types (α : TA → PROP) (β : TA → TB → PROP) (Ψ : PROP).
+  Context `{!irisGS_gen hlc Λ Σ} {TA TB : tele}.
+  Notation iProp := (iProp Σ).
+  Implicit Types (α : TA → iProp) (β : TA → TB → iProp) (Φ : TA → TB → iProp) (Ψ : iProp).
 
   Lemma ainv_intro Eo Ei α β Φ :
     Ei ⊆ Eo →
@@ -49,14 +118,14 @@ Section properties.
 
   Lemma ainv_ainv_frame {TA' TB' : tele} E1 E1' E2 E3
         α β Φ R
-        (α' : TA' → PROP) (β' Φ' : TA' → TB' → PROP) :
+        (α' : TA' → iProp) (β' Φ' : TA' → TB' → iProp) :
     E1' ⊆ E1 → E3 ⊆ E2 →
     atomic_invariant E1' E2 α β Φ -∗
     R -∗
     (□ ∀.. x, α x ={E2}=∗ ∃.. x', α' x' ∗ (
       (α' x' -∗ α x) ∧ (∀.. y', β' x' y' ={E2}=∗ R -∗
         (α x ∗ (atomic_invariant E1' E2 α β Φ ={E1}=∗ Φ' x' y')) ∨
-        (∃.. y, β x y ∗ (atomic_resource E1' E2 α Φ x y ={E1}=∗ Φ' x' y')))
+        (∃.. y, β x y ∗ (atomic_resource E1' E2 α (Φ x y) ={E1}=∗ Φ' x' y')))
     )) -∗
     atomic_invariant E1 E3 α' β' Φ'.
   Proof.
@@ -89,18 +158,17 @@ Section properties.
           iModIntro. iFrame. iIntros. iModIntro. iFrame.
         * iIntros (?) "Hα'". iDestruct ("Hα" with "Hα'") as "Hα".
           iModIntro. rewrite ->!tele_app_bind. iFrame.
-          iLeft. iIntros. by iApply "HΦ'".
   Qed.
 
   Lemma ainv_ainv {TA' TB' : tele} E1 E1' E2 E3
         α β Φ
-        (α' : TA' → PROP) (β' Φ' : TA' → TB' → PROP) :
+        (α' : TA' → iProp) (β' Φ' : TA' → TB' → iProp) :
     E1' ⊆ E1 → E3 ⊆ E2 →
     atomic_invariant E1' E2 α β Φ -∗
     (□ ∀.. x, α x ={E2}=∗ ∃.. x', α' x' ∗ (
       (α' x' -∗ α x) ∧ (∀.. y', β' x' y' ={E2}=∗
         (α x ∗ (atomic_invariant E1' E2 α β Φ ={E1}=∗ Φ' x' y')) ∨
-        (∃.. y, β x y ∗ (atomic_resource E1' E2 α Φ x y ={E1}=∗ Φ' x' y')))
+        (∃.. y, β x y ∗ (atomic_resource E1' E2 α (Φ x y) ={E1}=∗ Φ' x' y')))
     )) -∗
     atomic_invariant E1 E3 α' β' Φ'.
   Proof.
@@ -115,23 +183,23 @@ Section properties.
     iMod ("HΦ'" with "Hβ'") as "HΦ'". iModIntro. by iIntros.
   Qed.
 
-  Lemma ares_commit Eo Ei α Φ x (y : TB) :
-    atomic_resource Eo Ei α Φ x y ={Eo}=∗ Φ x y.
+  Lemma ares_commit Eo Ei α Ψ :
+    atomic_resource Eo Ei α Ψ ={Eo}=∗ Ψ.
   Proof.
     iIntros ">[%z [Hα [_ Hclose]]]".
-    iMod ("Hclose" $! y with "Hα") as "HΦ".
+    iMod ("Hclose" $! z with "Hα") as "HΦ".
     by iModIntro.
   Qed.
 
   Lemma ainv_ares_frame {TA' TB' : tele} E1 E1' E2 E3
-        α Φ z (y : TB) R
-        (α' : TA' → PROP) (β' Φ' : TA' → TB' → PROP) :
+        α Ψ R
+        (α' : TA' → iProp) (β' Φ' : TA' → TB' → iProp) :
     E1' ⊆ E1 → E3 ⊆ E2 →
-    atomic_resource E1' E2 α Φ z y -∗
+    atomic_resource E1' E2 α Ψ -∗
     R -∗
     (□ ∀.. x, α x ={E2}=∗ ∃.. x', α' x' ∗ (
       (α' x' -∗ α x) ∧ (∀.. y', β' x' y' ={E2}=∗ R -∗
-        α x ∗ (atomic_resource E1' E2 α Φ z y ={E1}=∗ Φ' x' y'))
+        α x ∗ (atomic_resource E1' E2 α Ψ ={E1}=∗ Φ' x' y'))
     )) -∗
     atomic_invariant E1 E3 α' β' Φ'.
   Proof.
@@ -158,13 +226,13 @@ Section properties.
   Qed.
 
   Lemma ainv_ares {TA' TB' : tele} E1 E1' E2 E3
-        α Φ z (y : TB)
-        (α' : TA' → PROP) (β' Φ' : TA' → TB' → PROP) :
+        α Ψ
+        (α' : TA' → iProp) (β' Φ' : TA' → TB' → iProp) :
     E1' ⊆ E1 → E3 ⊆ E2 →
-    atomic_resource E1' E2 α Φ z y -∗
+    atomic_resource E1' E2 α Ψ -∗
     (□ ∀.. x, α x ={E2}=∗ ∃.. x', α' x' ∗ (
       (α' x' -∗ α x) ∧ (∀.. y', β' x' y' ={E2}=∗
-        α x ∗ (atomic_resource E1' E2 α Φ z y ={E1}=∗ Φ' x' y'))
+        α x ∗ (atomic_resource E1' E2 α Ψ ={E1}=∗ Φ' x' y'))
     )) -∗
     atomic_invariant E1 E3 α' β' Φ'.
   Proof.
@@ -177,5 +245,43 @@ Section properties.
     iSplit; first by iDestruct "HΦ'" as "[$ _]".
     iDestruct "HΦ'" as "[_ HΦ']". iIntros (y') "Hβ'".
     iMod ("HΦ'" with "Hβ'") as "HΦ'". iModIntro. by iIntros.
+  Qed.
+
+  Lemma atomic_invariant_mask_weaken Eo1 Eo2 Ei α β Φ :
+    Eo1 ⊆ Eo2 →
+    atomic_invariant Eo1 Ei α β Φ -∗ atomic_invariant Eo2 Ei α β Φ.
+  Proof.
+    iIntros (HE) "AI".
+    iApply (ainv_ainv with "AI"); try done.
+    iIntros "!>" (x) "Hα". iModIntro. iExists x. iFrame.
+    iSplit; first by iIntros. iIntros (y) "Hβ".
+    iModIntro. iRight. iExists y. iFrame.
+    iIntros ">[%z [Hα [_ Hclose]]]".
+    by iApply ("Hclose" $! z).
+  Qed.
+
+  Lemma atomic_invariant_inv Eo Ei α β Φ N I :
+    ↑N ⊆ Eo →
+    atomic_invariant (Eo ∖ ↑N) Ei α β Φ -∗ inv N I -∗
+    atomic_invariant Eo Ei (λ.. x, ▷ I ∗ α x) (λ.. x y, ▷ I ∗ β x y) Φ.
+  Proof.
+    intros ?. iIntros "AI #Hinv".
+    iApply ainv_aupd. iAuIntro. iInv N as "HI".
+    iApply (aacc_aupd with "AI"); first solve_ndisj.
+    iIntros (x) "Hα". iAaccIntro with "[HI Hα]"; rewrite ->!tele_app_bind; first by iFrame.
+    - (* abort *)
+      iIntros "[HI $]". by eauto with iFrame.
+    - (* commit *)
+      iIntros (y). rewrite ->!tele_app_bind. iIntros "[HI Hβ]".
+      iModIntro. iRight. iExists y. iFrame. iIntros "AU".
+      iModIntro. iApply ares_aupd. iAuIntro. iInv N as "HI".
+      iApply (aacc_aupd with "AU"); first solve_ndisj.
+      iIntros (z) "Hα". iAaccIntro with "[HI Hα]";
+        rewrite ->!tele_app_bind; first by iFrame.
+      * iIntros "[HI $]". iModIntro. iIntros "AU".
+        iModIntro. iFrame.
+      * iIntros (w) "[HI Hα]". iModIntro.
+        rewrite ->!tele_app_bind. iRight.
+        iExists w. iFrame. by iIntros.
   Qed.
 End properties.
